lean/dk_math/DkMath/FLT/Seven.lean
@@ -70,6 +70,7 @@ import DkMath.FLT.Seven.SevenRealCubicCurrentCoefficientPhaseCollapse
 import DkMath.FLT.Seven.SevenRealCubicCurrentQuotientGapOrientation
 import DkMath.FLT.Seven.SevenRealCubicCurrentResidueKernel
 import DkMath.FLT.Seven.SevenRealCubicCurrentOrientationRatio
+import DkMath.FLT.Seven.SevenRealCubicCurrentPhaseCorrectedCarrier
 import DkMath.FLT.Seven.SevenRealCubicCurrentKummerPhaseSieve
 import DkMath.FLT.Seven.PrimeTraceOneDirectRealCubicSharpenedBranch
 import DkMath.FLT.Seven.SevenRealCubicSourcePlaneNormSeven
